ver2/memory_ops_solvers.v
@@ -33,7 +33,7 @@ Import ValidSymbolicState.
 
 Module MemoryOpsSolvers.
 
-(* sv smem instk_height m ops -> load_res *)
+(* sv smem instk_height m ops -> smap_value *)
 Definition mload_solver_type := sstack_val -> smemory -> nat -> smap -> stack_op_instr_map -> smap_value.
             
 Definition mload_solver_valid_res (mload_solver: mload_solver_type) :=
