ver2/symbolic_state_eval_facts.v
@@ -1,4 +1,4 @@
-Require Import Arith. 
+Require Import Arith.
 Require Import Nat.
 Require Import Bool.
 Require Import bbv.Word.
@@ -38,7 +38,6 @@ Import SymbolicStateEval.
 (*
 Fixpoint eval_sstack_val (sv : sstack_val) (stk : stack) (mem: memory) (strg: storage) (ctx: context) (maxidx: nat) (sb: sbindings) (ops: stack_op_instr_map) : option EVMWord :=  
 *)
- 
 
 Lemma n_Sm_neq_lt:
   forall n m,
@@ -61,78 +60,198 @@ Proof.
   apply H.
 Qed.
 
-  
-Lemma eval_sstack_val_succ:
-  forall sb instk_height sv stk mem strg ctx maxidx ops,
+
+Lemma valid_follow_in_smap:
+  forall sb sv instk_height maxidx ops smv maxidx' sb',
+    valid_sstack_value instk_height maxidx sv ->
+    valid_bindings instk_height maxidx sb ops ->
+    follow_in_smap sv maxidx sb = Some (FollowSmapVal smv maxidx' sb') ->
+    valid_smap_value instk_height maxidx' ops smv /\
+      valid_bindings instk_height maxidx' sb' ops /\
+      (not_basic_value_smv smv = true -> maxidx > maxidx').
+Proof.
+  induction sb as [|p sb'' IHsb''].
+  - intros sv instk_height maxidx ops smv maxidx' sb' H_valid_sv H_valid_sb H_follow.
+    destruct sv eqn:E_sv.
+    + simpl in H_valid_sv.
+      simpl in H_valid_sb.
+      simpl in H_follow.
+      injection H_follow as H_smv H_maxidx' H_sb'.
+      rewrite <- H_sb'.
+      rewrite <- H_smv.
+      rewrite <- H_maxidx'.
+      simpl.
+      split; try intuition.
+      
+    + simpl in H_valid_sv.
+      simpl in H_valid_sb.
+      simpl in H_follow.
+      injection H_follow as H_smv H_maxidx' H_sb'.
+      rewrite <- H_sb'.
+      rewrite <- H_smv.
+      rewrite <- H_maxidx'.
+      simpl.
+      split; try intuition.
+    + discriminate.
+  - intros sv instk_height maxidx ops smv maxidx' sb' H_valid_sv H_valid_sb H_follow.
+    destruct sv eqn:E_sv.
+    + simpl in H_valid_sv.
+      simpl in H_valid_sb.
+      simpl in H_follow.
+      injection H_follow as H_smv H_maxidx' H_sb'.
+      rewrite <- H_sb'.
+      rewrite <- H_smv.
+      rewrite <- H_maxidx'.
+      simpl.
+      split; try intuition.
+    + simpl in H_valid_sv.
+      simpl in H_valid_sb.
+      simpl in H_follow.
+      injection H_follow as H_smv H_maxidx' H_sb'.
+      rewrite <- H_sb'.
+      rewrite <- H_smv.
+      rewrite <- H_maxidx'.
+      simpl.
+      split; try intuition.
+    + destruct p as [idx value] eqn:E_p.
+      simpl in H_valid_sv.
+      simpl in H_valid_sb.
+      simpl in H_follow.
+      destruct H_valid_sb as [H_valid_sb_0 [H_valid_sb_1 H_valid_sb_2]].
+      destruct (idx =? var) eqn:E_n_var.
+      * destruct (is_fresh_var_smv value) as [idx'|] eqn:E_is_fresh_var_value.
+        ** destruct value eqn:E_value; try discriminate.
+           destruct val; try discriminate.
+           simpl in E_is_fresh_var_value.
+           injection E_is_fresh_var_value as E_is_fresh_var_value.
+           simpl in H_valid_sb_1.
+           rewrite E_is_fresh_var_value in H_valid_sb_1.
+
+           assert(H_valid_sstack_value_FreshVar_idx': valid_sstack_value instk_height idx (FreshVar idx')). intuition.
+
+           pose proof (IHsb'' (FreshVar idx') instk_height idx ops smv maxidx' sb' H_valid_sstack_value_FreshVar_idx' H_valid_sb_2 H_follow) as IHsb''_0.
+           intuition.
+           
+        ** injection H_follow as  H_value H_idx H_sb''.
+           rewrite <- H_idx.
+           rewrite <- H_sb''.
+           rewrite <- H_value.
+           split.
+           *** apply H_valid_sb_1.
+           *** split.
+               ***** apply H_valid_sb_2.
+               ***** intro H_not_basic_value.
+               destruct value; try intuition.
+      * apply Nat.eqb_neq in E_n_var.
+        assert(H_valid_sstack_value_FreshVar_idx': valid_sstack_value instk_height idx (FreshVar var)). simpl. intuition.
+        pose proof (IHsb'' (FreshVar var) instk_height idx ops smv maxidx' sb' H_valid_sstack_value_FreshVar_idx' H_valid_sb_2 H_follow) as IHsb''_0.
+        intuition.
+Qed.
+
+Lemma follow_in_smap_suc:
+  forall sb sv instk_height maxidx ops,
+    valid_sstack_value instk_height maxidx sv ->
+    valid_bindings instk_height maxidx sb ops ->
+    exists smv maxidx' sb',
+      follow_in_smap sv maxidx sb = Some (FollowSmapVal smv maxidx' sb') /\
+      is_fresh_var_smv smv = None.
+Proof.
+  induction sb as [| p sb' IHsb'].
+  - intros sv instk_height maxidx ops H_valid_sv H_valid_bs.
+    destruct sv eqn:E_sv.
+    + simpl. exists (SymBasicVal (Val val)). exists maxidx. exists [].
+      split; try reflexivity.
+    + simpl. exists (SymBasicVal (InStackVar var)). exists maxidx. exists [].
+      split; try reflexivity.
+    + simpl in H_valid_bs.
+      simpl in H_valid_sv.
+      intuition.
+  - intros sv instk_height maxidx ops H_valid_sv H_valid_bs.
+    destruct sv eqn:E_sv.
+    + simpl. exists (SymBasicVal (Val val)). exists maxidx. exists (p :: sb'). split; try reflexivity.
+    + simpl. exists (SymBasicVal (InStackVar var)). exists maxidx. exists (p :: sb'). split; try reflexivity.
+    + destruct p as [key value].      
+      simpl in H_valid_bs.
+      destruct H_valid_bs as [H_valid_bs_0 [H_valid_bs_1 H_valid_bs_2]].
+      simpl in H_valid_sv.
+      simpl.
+      destruct (key =? var) eqn:E_key_var.
+      * destruct (is_fresh_var_smv value) as [idx'|] eqn:E_is_fresh_var_smv_value.
+        ** apply IHsb' with (instk_height:=instk_height)(ops:=ops).
+           *** simpl.
+               destruct value; try discriminate.
+               simpl in E_is_fresh_var_smv_value.
+               destruct val; try discriminate.
+               injection E_is_fresh_var_smv_value as E_is_fresh_var_smv_value.
+               simpl in H_valid_bs_1.
+               intuition.
+           *** apply H_valid_bs_2.
+        ** exists value. exists key. exists sb'.
+           split; try reflexivity.
+           apply E_is_fresh_var_smv_value.
+      * apply IHsb' with (instk_height:=instk_height)(ops:=ops).
+        ** simpl.
+           apply Nat.eqb_neq in E_key_var. intuition.
+        ** apply H_valid_bs_2.
+Qed.
+
+Lemma eval_sstack_val'_succ:
+  forall d instk_height sv stk mem strg ctx maxidx sb ops,
     instk_height = length stk ->
     valid_sstack_value instk_height maxidx sv ->
     valid_bindings instk_height maxidx sb ops ->
+    d > maxidx ->
     exists v,
-      eval_sstack_val sv stk mem strg ctx maxidx sb ops = Some v.
+      eval_sstack_val' d sv stk mem strg ctx maxidx sb ops = Some v.
 Proof.
-  induction sb as [|p sb'].
-  - intros instk_height sv stk mem strg ctx maxidx ops H_instk_height H_valid_sv H_valid_sb.
-    destruct sv as [val|n|idx] eqn:E_svn.
-    + simpl. exists val. reflexivity.
-    + simpl. unfold valid_sstack_value in H_valid_sv.
-      rewrite H_instk_height in H_valid_sv. 
-      pose proof (nth_error_nth' stk WZero H_valid_sv) as H_nth_error_stk.
-      rewrite H_nth_error_stk.
-      exists (nth n stk WZero).
-      reflexivity.
-    + simpl.
-      simpl valid_bindings in H_valid_sb.
-      simpl in H_valid_sv.
-      rewrite H_valid_sb in H_valid_sv.
-      pose proof Nat.nlt_0_r idx.
-      contradiction.
-  - intros instk_height sv stk mem strg ctx maxidx ops H_instk_height H_valid_sv H_valid_sb.
-    destruct sv as [val|n|idx] eqn:E_sv.
+  induction d as [|d' IHd'].
+  - intros instk_height sv stk mem strg ctx maxidx sb ops H_instk_height H_valid_sv H_valid_sb H_d_S_maxid.
+    apply Nat.nlt_0_r in H_d_S_maxid.
+    contradiction.
+    
+    
+  - intros instk_height sv stk mem strg ctx maxidx sb ops H_instk_height H_valid_sv H_valid_sb H_d_S_maxid.
 
-    (* Val *)
-    + simpl. exists val. reflexivity.
+    unfold eval_sstack_val'. fold eval_sstack_val'.
+    
+    pose proof (follow_in_smap_suc sb sv instk_height maxidx ops H_valid_sv H_valid_sb) as H_follow.
+    destruct H_follow as [smv [maxidx' [sb' H_follow]]].
+    destruct H_follow as [H_follow_1 H_follow_2].
+    pose proof (valid_follow_in_smap sb sv instk_height maxidx ops smv maxidx' sb' H_valid_sv H_valid_sb H_follow_1) as H_follow_valid.
 
-    (* InStackVar *)
-    + simpl. unfold valid_sstack_value in H_valid_sv.
-      rewrite H_instk_height in H_valid_sv. 
-      pose proof (nth_error_nth' stk WZero H_valid_sv) as H_nth_error_stk.
-      rewrite H_nth_error_stk.
-      exists (nth n stk WZero).
-      reflexivity.
+    destruct H_follow_valid as [H_follow_valid_0 [H_follow_valid_1 H_follow_valid_2]].
+    rewrite H_follow_1.
 
-    (* FreshVar *)
-    + simpl.
-      fold eval_sstack_val.
-      destruct p as [key smv].
-      destruct (key =? idx) eqn:E_key_eqb_idx.
+    destruct smv as [sv' | v | label args | soffset smem | skey sstrg | soffset ssize smem ] eqn:E_smv.
 
-      (* idx is equal to key *)
-      * destruct smv as [sv' | v | label args | soffset smem | skey sstrg | soffset ssize smem ] eqn:E_smv.
+    (* SymBasicVal *)
+    ** destruct sv' as [val | var | idx' ] eqn:E_sv'.
+       *** exists val. reflexivity.
+       *** simpl in H_follow_valid_0.
+           rewrite H_instk_height in H_follow_valid_0.
+           apply nth_error_nth' with (d:=WZero) in H_follow_valid_0.
+           rewrite H_follow_valid_0.
+           exists (nth var stk WZero).
+           reflexivity.
+       *** discriminate H_follow_2.
 
-        (* SymBasicVal *)
-        ** unfold valid_bindings in H_valid_sb. fold valid_bindings in H_valid_sb.
-           destruct H_valid_sb as [H_valid_sb_0 [H_valid_sb_1 H_valid_sb_2]].
-           unfold valid_smap_value in H_valid_sb_1.
-           pose proof (IHsb' instk_height sv' stk mem strg ctx key ops H_instk_height H_valid_sb_1 H_valid_sb_2) as IHsb'_0.
-           apply IHsb'_0.
+    (* SymPUSHTAG  *)
+    ** exists (get_tags_ctx ctx v). reflexivity.
+       
+    (* OpImp nargs f *)
+    ** destruct (ops label) eqn:E_f.
+       unfold valid_bindings in H_valid_sb. fold valid_bindings in H_valid_sb.
+       simpl in H_follow_valid_0.
+       unfold valid_stack_op_instr in H_follow_valid_0.
+       rewrite E_f in H_follow_valid_0.
+       destruct H_follow_valid_0 as [H_follow_valid_0_0 H_follow_valid_0_1].
+       apply Nat.eqb_eq in H_follow_valid_0_0 as H_follow_valid_0_0_eqb.
+       rewrite H_follow_valid_0_0_eqb.
+       fold eval_sstack_val'.
 
-        (* SymPUSHTAG  *)
-        ** exists (get_tags_ctx ctx v). reflexivity.
-
-        (* OpImp nargs f *)
-        ** destruct (ops label) eqn:E_f.
-           unfold valid_bindings in H_valid_sb. fold valid_bindings in H_valid_sb.
-           destruct H_valid_sb as [H_valid_sb_0 [H_valid_sb_1 H_valid_sb_2]].
-           unfold valid_smap_value in H_valid_sb_1.
-           unfold valid_stack_op_instr in H_valid_sb_1.
-           rewrite E_f in H_valid_sb_1.
-           destruct H_valid_sb_1 as [H_valid_sb_1_0 H_valid_sb_1_1].
-           apply Nat.eqb_eq in H_valid_sb_1_0 as H_valid_sb_1_0_eqb.
-           rewrite H_valid_sb_1_0_eqb.
-
-           assert(H_eval_args: forall args0,
-                     valid_sstack instk_height key args0 ->
-                     exists v, map_option (fun sv' : sstack_val => eval_sstack_val sv' stk mem strg ctx key sb' ops) args0 = Some v).
+       assert(H_eval_args: forall args0,
+                 valid_sstack instk_height maxidx' args0 ->
+                 exists v, map_option (fun sv' : sstack_val => eval_sstack_val' d' sv' stk mem strg ctx maxidx' sb' ops) args0 = Some v).
            (* proof of assert *)
            *** induction args0 as [|a args0' IHargs'].
                **** intros. exists []. reflexivity.
@@ -141,9 +260,10 @@ Proof.
                     destruct H_valid_args0 as [H_valid_a H_valid_args0].
                     unfold map_option.
                     rewrite <- map_option_ho.
-                    pose proof (IHsb' instk_height a stk mem strg ctx key ops H_instk_height H_valid_a H_valid_sb_2) as IHsb'_0.
-                    destruct IHsb'_0 as [v IHsb'_0].
-                    rewrite IHsb'_0.
+                    assert (H_d'_gt_maxidx': d' > maxidx'). intuition.
+                    pose proof (IHd' instk_height a stk mem strg ctx maxidx' sb' ops H_instk_height H_valid_a H_follow_valid_1 H_d'_gt_maxidx') as IHd'_0.
+                    destruct IHd'_0 as [v IHd'_0].
+                    rewrite IHd'_0.
                     pose proof  IHargs'  H_valid_args0 as IHargs'_0.
                     destruct IHargs'_0 as [vargs0' IHargs'_0].
                     rewrite IHargs'_0.
@@ -151,23 +271,21 @@ Proof.
                     reflexivity.
            (* end proof of assert *)
 
-           *** pose proof (H_eval_args args H_valid_sb_1_1) as H_eval_args.
+           *** pose proof (H_eval_args args H_follow_valid_0_1) as H_eval_args.
                destruct H_eval_args as [v H_eval_args].
                rewrite H_eval_args.
                exists (f ctx v).
                reflexivity.
 
         (* SymMLOAD *)
-        ** unfold valid_bindings in H_valid_sb. fold valid_bindings in H_valid_sb.
-           destruct H_valid_sb as [H_valid_sb_0 [H_valid_sb_1 H_valid_sb_2]].
-           unfold valid_smap_value in H_valid_sb_1.
-           destruct H_valid_sb_1 as [H_valid_sb_1_0 H_valid_sb_1_1].
+    ** unfold valid_smap_value in H_follow_valid_0.
+       destruct H_follow_valid_0 as [H_valid_sb_1_0 H_valid_sb_1_1].
 
-           assert(H_map_o_smem:
-                   forall smem0,
-                     valid_smemory instk_height key smem0 ->
-                     exists v,
-                       map_option (eval_common.EvalCommon.instantiate_memory_update (fun sv0 : sstack_val => eval_sstack_val sv0 stk mem strg ctx key sb' ops)) smem0 = Some v).
+       assert(H_map_o_smem:
+               forall smem0,
+                 valid_smemory instk_height maxidx' smem0 ->
+                 exists v,
+                   map_option (eval_common.EvalCommon.instantiate_memory_update (fun sv0 : sstack_val => eval_sstack_val' d' sv0 stk mem strg ctx maxidx' sb' ops)) smem0 = Some v).
 
            (* proof of assert *)
            *** induction smem0 as [|u smem0' IHsmem0'].
@@ -182,12 +300,14 @@ Proof.
                           destruct H_valid_smemory as [H_valid_smemory_0 H_valid_smemory_1].
                           unfold valid_smemory_update in H_valid_smemory_0.
                           destruct H_valid_smemory_0 as [H_valid_smemory_0_0 H_valid_smemory_0_1].
-                          pose proof (IHsb' instk_height soffset' stk mem strg ctx key ops H_instk_height H_valid_smemory_0_0 H_valid_sb_2) as IHsb'_0.
-                          destruct IHsb'_0 as [voffset IHsb'_0].
-                          rewrite  IHsb'_0.
-                          pose proof (IHsb' instk_height svalue' stk mem strg ctx key ops H_instk_height H_valid_smemory_0_1 H_valid_sb_2) as IHsb'_1.
-                          destruct IHsb'_1 as [vvalue IHsb'_1].
-                          rewrite  IHsb'_1.
+                          
+                          assert (H_d'_gt_maxidx': d' > maxidx'). intuition.
+                          pose proof (IHd' instk_height soffset' stk mem strg ctx maxidx' sb' ops H_instk_height H_valid_smemory_0_0 H_follow_valid_1 H_d'_gt_maxidx') as IHd'_0.
+                          destruct IHd'_0 as [voffset IHd'_0].
+                          rewrite IHd'_0.
+                          pose proof (IHd' instk_height svalue' stk mem strg ctx maxidx' sb' ops H_instk_height H_valid_smemory_0_1 H_follow_valid_1 H_d'_gt_maxidx') as IHd'_1.
+                          destruct IHd'_1 as [vvalue IHd'_1].
+                          rewrite  IHd'_1.
 
                           pose proof (IHsmem0' H_valid_smemory_1) as IHsmem0'_0.
                           destruct IHsmem0'_0 as [vsmem0' IHsmem0'_0].
@@ -198,12 +318,14 @@ Proof.
                           destruct H_valid_smemory as [H_valid_smemory_0 H_valid_smemory_1].
                           unfold valid_smemory_update in H_valid_smemory_0.
                           destruct H_valid_smemory_0 as [H_valid_smemory_0_0 H_valid_smemory_0_1].
-                          pose proof (IHsb' instk_height soffset' stk mem strg ctx key ops H_instk_height H_valid_smemory_0_0 H_valid_sb_2) as IHsb'_0.
-                          destruct IHsb'_0 as [voffset IHsb'_0].
-                          rewrite  IHsb'_0.
-                          pose proof (IHsb' instk_height svalue' stk mem strg ctx key ops H_instk_height H_valid_smemory_0_1 H_valid_sb_2) as IHsb'_1.
-                          destruct IHsb'_1 as [vvalue IHsb'_1].
-                          rewrite  IHsb'_1.
+                          
+                          assert (H_d'_gt_maxidx': d' > maxidx'). intuition.
+                          pose proof (IHd' instk_height soffset' stk mem strg ctx maxidx' sb' ops H_instk_height H_valid_smemory_0_0 H_follow_valid_1 H_d'_gt_maxidx') as IHd'_0.
+                          destruct IHd'_0 as [voffset IHd'_0].
+                          rewrite IHd'_0.
+                          pose proof (IHd' instk_height svalue' stk mem strg ctx maxidx' sb' ops H_instk_height H_valid_smemory_0_1 H_follow_valid_1 H_d'_gt_maxidx') as IHd'_1.
+                          destruct IHd'_1 as [vvalue IHd'_1].
+                          rewrite  IHd'_1.
 
                           pose proof (IHsmem0' H_valid_smemory_1) as IHsmem0'_0.
                           destruct IHsmem0'_0 as [vsmem0' IHsmem0'_0].
@@ -216,24 +338,23 @@ Proof.
                destruct H_map_o_smem_0 as [v H_map_o_smem_0].
                rewrite H_map_o_smem_0.
 
-               pose proof (IHsb' instk_height soffset stk mem strg ctx key ops H_instk_height H_valid_sb_1_0 H_valid_sb_2) as IHsb'_0.
-               destruct IHsb'_0 as [voffset IHsb'_0].
-               rewrite IHsb'_0.
+               assert (H_d'_gt_maxidx': d' > maxidx'). intuition.
+               pose proof (IHd' instk_height soffset stk mem strg ctx maxidx' sb' ops H_instk_height H_valid_sb_1_0 H_follow_valid_1 H_d'_gt_maxidx') as IHd'_0.
+               destruct IHd'_0 as [voffset IHd'_0].
+               rewrite IHd'_0.
 
                exists (concrete_interpreter.ConcreteInterpreter.mload (eval_common.EvalCommon.update_memory mem v) voffset).
                reflexivity.
 
-        (* SymMLOAD *)
-        ** unfold valid_bindings in H_valid_sb. fold valid_bindings in H_valid_sb.
-           destruct H_valid_sb as [H_valid_sb_0 [H_valid_sb_1 H_valid_sb_2]].
-           unfold valid_smap_value in H_valid_sb_1.
-           destruct H_valid_sb_1 as [H_valid_sb_1_0 H_valid_sb_1_1].
+        (* SymSLOAD *)
+        ** unfold valid_smap_value in H_follow_valid_0.
+           destruct H_follow_valid_0 as [H_valid_sb_1_0 H_valid_sb_1_1].
 
            assert(H_map_o_sstrg:
                    forall sstrg0,
-                     valid_sstorage instk_height key sstrg0 ->
+                     valid_sstorage instk_height maxidx' sstrg0 ->
                      exists v,
-                       map_option (eval_common.EvalCommon.instantiate_storage_update (fun sv0 : sstack_val => eval_sstack_val sv0 stk mem strg ctx key sb' ops)) sstrg0 = Some v).
+                       map_option (eval_common.EvalCommon.instantiate_storage_update (fun sv0 : sstack_val => eval_sstack_val' d' sv0 stk mem strg ctx maxidx' sb' ops)) sstrg0 = Some v).
            
            (* proof of assert *)
            *** induction sstrg0 as [|u sstrg0' IHsstrg0'].
@@ -248,12 +369,15 @@ Proof.
                     destruct H_valid_sstorage as [H_valid_sstorage_0 H_valid_sstorage_1].
                     unfold valid_sstorage_update in H_valid_sstorage_0.
                     destruct H_valid_sstorage_0 as [H_valid_sstorage_0_0 H_valid_sstorage_0_1].
-                    pose proof (IHsb' instk_height skey' stk mem strg ctx key ops H_instk_height H_valid_sstorage_0_0 H_valid_sb_2) as IHsb'_0.
-                    destruct IHsb'_0 as [voffset IHsb'_0].
-                    rewrite  IHsb'_0.
-                    pose proof (IHsb' instk_height svalue' stk mem strg ctx key ops H_instk_height H_valid_sstorage_0_1 H_valid_sb_2) as IHsb'_1.
-                    destruct IHsb'_1 as [vvalue IHsb'_1].
-                    rewrite  IHsb'_1.
+
+                    assert (H_d'_gt_maxidx': d' > maxidx'). intuition.
+                    pose proof (IHd' instk_height skey' stk mem strg ctx maxidx' sb' ops H_instk_height H_valid_sstorage_0_0 H_follow_valid_1 H_d'_gt_maxidx') as IHd'_0.
+                    destruct IHd'_0 as [voffset IHd'_0].
+                    rewrite  IHd'_0.
+                    
+                    pose proof (IHd' instk_height svalue' stk mem strg ctx maxidx' sb' ops H_instk_height H_valid_sstorage_0_1 H_follow_valid_1 H_d'_gt_maxidx') as IHd'_1.
+                    destruct IHd'_1 as [vvalue IHd'_1].
+                    rewrite  IHd'_1.
                     
                     pose proof (IHsstrg0' H_valid_sstorage_1) as IHsstrg0'_0.
                     destruct IHsstrg0'_0 as [vsstrg0' IHsstrg0'_0].
@@ -266,24 +390,23 @@ Proof.
                destruct H_map_o_sstrg_0 as [v H_map_o_sstrg_0].
                rewrite H_map_o_sstrg_0.
 
-               pose proof (IHsb' instk_height skey stk mem strg ctx key ops H_instk_height H_valid_sb_1_0 H_valid_sb_2) as IHsb'_0.
-               destruct IHsb'_0 as [vkey IHsb'_0].
-               rewrite IHsb'_0.
+               assert (H_d'_gt_maxidx': d' > maxidx'). intuition.
+               pose proof (IHd' instk_height skey stk mem strg ctx maxidx' sb' ops H_instk_height H_valid_sb_1_0 H_follow_valid_1 H_d'_gt_maxidx') as IHd'_0.
+               destruct IHd'_0 as [vkey IHd'_0].
+               rewrite IHd'_0.
 
                exists (concrete_interpreter.ConcreteInterpreter.sload (eval_common.EvalCommon.update_storage strg v) vkey).
                reflexivity.
 
         (* SymSHA3 *)
-        ** unfold valid_bindings in H_valid_sb. fold valid_bindings in H_valid_sb.
-           destruct H_valid_sb as [H_valid_sb_0 [H_valid_sb_1 H_valid_sb_2]].
-           unfold valid_smap_value in H_valid_sb_1.
-           destruct H_valid_sb_1 as [H_valid_sb_1_0 [H_valid_sb_1_1 H_valid_sb_1_2]].
-
+        ** unfold valid_smap_value in H_follow_valid_0.
+           destruct H_follow_valid_0 as [H_valid_sb_1_0 [H_valid_sb_1_1 H_valid_sb_1_2]].
+           
            assert(H_map_o_smem:
-                   forall smem0,
-                     valid_smemory instk_height key smem0 ->
-                     exists v,
-                       map_option (eval_common.EvalCommon.instantiate_memory_update (fun sv0 : sstack_val => eval_sstack_val sv0 stk mem strg ctx key sb' ops)) smem0 = Some v).
+               forall smem0,
+                 valid_smemory instk_height maxidx' smem0 ->
+                 exists v,
+                   map_option (eval_common.EvalCommon.instantiate_memory_update (fun sv0 : sstack_val => eval_sstack_val' d' sv0 stk mem strg ctx maxidx' sb' ops)) smem0 = Some v).
 
            (* proof of assert *)
            *** induction smem0 as [|u smem0' IHsmem0'].
@@ -298,12 +421,14 @@ Proof.
                           destruct H_valid_smemory as [H_valid_smemory_0 H_valid_smemory_1].
                           unfold valid_smemory_update in H_valid_smemory_0.
                           destruct H_valid_smemory_0 as [H_valid_smemory_0_0 H_valid_smemory_0_1].
-                          pose proof (IHsb' instk_height soffset' stk mem strg ctx key ops H_instk_height H_valid_smemory_0_0 H_valid_sb_2) as IHsb'_0.
-                          destruct IHsb'_0 as [voffset IHsb'_0].
-                          rewrite  IHsb'_0.
-                          pose proof (IHsb' instk_height svalue' stk mem strg ctx key ops H_instk_height H_valid_smemory_0_1 H_valid_sb_2) as IHsb'_1.
-                          destruct IHsb'_1 as [vvalue IHsb'_1].
-                          rewrite  IHsb'_1.
+                          
+                          assert (H_d'_gt_maxidx': d' > maxidx'). intuition.
+                          pose proof (IHd' instk_height soffset' stk mem strg ctx maxidx' sb' ops H_instk_height H_valid_smemory_0_0 H_follow_valid_1 H_d'_gt_maxidx') as IHd'_0.
+                          destruct IHd'_0 as [voffset IHd'_0].
+                          rewrite IHd'_0.
+                          pose proof (IHd' instk_height svalue' stk mem strg ctx maxidx' sb' ops H_instk_height H_valid_smemory_0_1 H_follow_valid_1 H_d'_gt_maxidx') as IHd'_1.
+                          destruct IHd'_1 as [vvalue IHd'_1].
+                          rewrite  IHd'_1.
 
                           pose proof (IHsmem0' H_valid_smemory_1) as IHsmem0'_0.
                           destruct IHsmem0'_0 as [vsmem0' IHsmem0'_0].
@@ -314,12 +439,14 @@ Proof.
                           destruct H_valid_smemory as [H_valid_smemory_0 H_valid_smemory_1].
                           unfold valid_smemory_update in H_valid_smemory_0.
                           destruct H_valid_smemory_0 as [H_valid_smemory_0_0 H_valid_smemory_0_1].
-                          pose proof (IHsb' instk_height soffset' stk mem strg ctx key ops H_instk_height H_valid_smemory_0_0 H_valid_sb_2) as IHsb'_0.
-                          destruct IHsb'_0 as [voffset IHsb'_0].
-                          rewrite  IHsb'_0.
-                          pose proof (IHsb' instk_height svalue' stk mem strg ctx key ops H_instk_height H_valid_smemory_0_1 H_valid_sb_2) as IHsb'_1.
-                          destruct IHsb'_1 as [vvalue IHsb'_1].
-                          rewrite  IHsb'_1.
+                          
+                          assert (H_d'_gt_maxidx': d' > maxidx'). intuition.
+                          pose proof (IHd' instk_height soffset' stk mem strg ctx maxidx' sb' ops H_instk_height H_valid_smemory_0_0 H_follow_valid_1 H_d'_gt_maxidx') as IHd'_0.
+                          destruct IHd'_0 as [voffset IHd'_0].
+                          rewrite IHd'_0.
+                          pose proof (IHd' instk_height svalue' stk mem strg ctx maxidx' sb' ops H_instk_height H_valid_smemory_0_1 H_follow_valid_1 H_d'_gt_maxidx') as IHd'_1.
+                          destruct IHd'_1 as [vvalue IHd'_1].
+                          rewrite  IHd'_1.
 
                           pose proof (IHsmem0' H_valid_smemory_1) as IHsmem0'_0.
                           destruct IHsmem0'_0 as [vsmem0' IHsmem0'_0].
@@ -332,32 +459,36 @@ Proof.
                destruct H_map_o_smem_0 as [v H_map_o_smem_0].
                rewrite H_map_o_smem_0.
 
-               pose proof (IHsb' instk_height soffset stk mem strg ctx key ops H_instk_height H_valid_sb_1_0 H_valid_sb_2) as IHsb'_0.
-               destruct IHsb'_0 as [voffset IHsb'_0].
-               rewrite IHsb'_0.
+               assert (H_d'_gt_maxidx': d' > maxidx'). intuition.
+               pose proof (IHd' instk_height soffset stk mem strg ctx maxidx' sb' ops H_instk_height H_valid_sb_1_0 H_follow_valid_1 H_d'_gt_maxidx') as IHd'_0.
+               destruct IHd'_0 as [voffset IHd'_0].
+               rewrite IHd'_0.
 
-               pose proof (IHsb' instk_height ssize stk mem strg ctx key ops H_instk_height H_valid_sb_1_1 H_valid_sb_2) as IHsb'_1.
-               destruct IHsb'_1 as [vsize IHsb'_1].
-               rewrite IHsb'_1.
+               pose proof (IHd' instk_height ssize stk mem strg ctx maxidx' sb' ops H_instk_height H_valid_sb_1_1 H_follow_valid_1 H_d'_gt_maxidx') as IHd'_1.
+               destruct IHd'_1 as [vsize IHd'_1].
+               rewrite IHd'_1.
 
                exists (get_keccak256_ctx ctx (wordToNat vsize) (concrete_interpreter.ConcreteInterpreter.mload' (eval_common.EvalCommon.update_memory mem v) voffset(wordToNat vsize))).
                reflexivity.
-
-      (* idx is different from key *)
-      * unfold valid_bindings in H_valid_sb.
-        fold valid_bindings in H_valid_sb.
-        destruct H_valid_sb as [H_valid_sb_0 [H_valid_sb_1 H_valid_sb_2]].
-        unfold valid_sstack_value in H_valid_sv.
-        apply Nat.eqb_neq in E_key_eqb_idx as E_key_neq_idx.
-        rewrite H_valid_sb_0 in H_valid_sv.
-        apply not_eq_sym in E_key_neq_idx.
-        pose proof (n_Sm_neq_lt idx key H_valid_sv E_key_neq_idx) as H_idx_lt_key.
-        pose proof (valid_sstack_value_FreshVar instk_height key idx H_idx_lt_key) as H_valid_sstack_value_FreshVar.
-        pose proof (IHsb' instk_height (FreshVar idx) stk mem strg ctx key ops H_instk_height H_valid_sstack_value_FreshVar H_valid_sb_2) as IHsb'_0.
-        apply IHsb'_0.
 Qed.
 
-
+  
+Lemma eval_sstack_val_succ:
+  forall sb instk_height sv stk mem strg ctx maxidx ops,
+    instk_height = length stk ->
+    valid_sstack_value instk_height maxidx sv ->
+    valid_bindings instk_height maxidx sb ops ->
+    exists v,
+      eval_sstack_val sv stk mem strg ctx maxidx sb ops = Some v.
+Proof.
+  intros sb instk_height sv stk mem strg ctx maxidx ops H_instk_height H_valid_sv H_valid_sb.
+  unfold eval_sstack_val.
+  assert (H_S_maxidx_gt_maxidx: S maxidx > maxidx ). auto.
+  pose proof (eval_sstack_val'_succ (S maxidx) instk_height sv stk mem strg ctx maxidx sb ops H_instk_height H_valid_sv H_valid_sb H_S_maxidx_gt_maxidx) as H_eval_sstack_val'_succ.
+  destruct H_eval_sstack_val'_succ as [v H_eval_sstack_val'_succ].
+  exists v.
+  apply H_eval_sstack_val'_succ.
+Qed.
 
   
 Lemma eval_map_o_sstk_succ:
